Define pre and post states for one of the add tests

vfmStateScript.sml
@@ -13,12 +13,31 @@ Datatype:
    |>
 End
 
+Definition empty_storage_def:
+  empty_storage: bytes32 -> bytes32 = K 0w
+End
+
 (* TODO: this probably needs to depend on block number (for hardforks) *)
 Definition wf_account_state_def:
   wf_account_state a
   ⇔ a.nonce < 2 ** 64                  (* https://eips.ethereum.org/EIPS/eip-2681 *)
   ∧ LENGTH a.code <= 2 ** 14 + 2 ** 13 (* https://eips.ethereum.org/EIPS/eip-170 *)
 End
+
+Definition empty_account_state_def:
+  empty_account_state =
+    <| nonce := 0
+     ; balance := 0
+     ; storage := empty_storage
+     ; code := []
+     |>
+End
+
+Theorem wf_empty_account_state[simp]:
+  wf_account_state empty_account_state
+Proof
+  rw[empty_account_state_def, wf_account_state_def]
+QED
 
 Type evm_accounts = “:address -> account_state”
 
