vfmTestScript.sml
@@ -11,6 +11,138 @@ Definition hex_to_bytes_def:
       :: hex_to_bytes rest
 End
 
+(* BlockchainTests/GeneralStateTests/VMTests/vmArithmeticTest/add.json *)
+
+Definition add_d0g0v0_Shanghai_transaction_def:
+  add_d0g0v0_Shanghai_transaction =
+  <| from := n2w 0xa94f5374fce5edbc8e2a8697c15331677e6ebf0b
+   ; to   := n2w 0xcccccccccccccccccccccccccccccccccccccccc
+   ; data := hex_to_bytes $ CONCAT [
+               "693c61390000000000000000000000000000";
+               "000000000000000000000000000000000000" ]
+   ; nonce := 0x00
+   ; value := 0x01
+   ; gasPrice := 0x0a
+   ; gasLimit := 0x04c4b400
+   ; accessList := []
+   |>
+End
+
+Definition add_d0g0v0_Shanghai_pre_def:
+  add_d0g0v0_Shanghai_pre a =
+  if a = n2w 0x0000000000000000000000000000000000001000 then
+    <| nonce := 0x00
+     ; balance := 0x0ba1a9ce0ba1a9ce
+     ; storage := empty_storage
+     ; code := hex_to_bytes $ CONCAT
+                 ["7ffffffffffffffffffffffffffffffffffffff"
+                 ;"fffffffffffffffffffffffffff7fffffffffff"
+                 ;"fffffffffffffffffffffffffffffffffffffff"
+                 ;"fffffffffffffff0160005500"]
+     |>
+  else if a = n2w 0x0000000000000000000000000000000000001001 then
+    <| nonce := 0x00
+     ; balance := 0x0ba1a9ce0ba1a9ce
+     ; storage := empty_storage
+     ; code := hex_to_bytes $ CONCAT
+                 ["60047fffffffffffffffffffffffffffffffffff"
+                 ;"ffffffffffffffffffffffffffffff0160005500"]
+     |>
+  else if a = n2w 0x0000000000000000000000000000000000001002 then
+    <| nonce := 0x00
+     ; balance := 0x0ba1a9ce0ba1a9ce
+     ; storage := empty_storage
+     ; code := hex_to_bytes $ CONCAT
+                 ["60017fffffffffffffffffffffffffffffffffff"
+                 ;"ffffffffffffffffffffffffffffff0160005500"]
+     |>
+  else if a = n2w 0x0000000000000000000000000000000000001003 then
+    <| nonce := 0x00
+     ; balance := 0x0ba1a9ce0ba1a9ce
+     ; storage := empty_storage
+     ; code := hex_to_bytes "600060000160005500"
+     |>
+  else if a = n2w 0x0000000000000000000000000000000000001004 then
+    <| nonce := 0x00
+     ; balance := 0x0ba1a9ce0ba1a9ce
+     ; storage := empty_storage
+     ; code := hex_to_bytes $ CONCAT
+                  ["7fffffffffffffffffffffffffffffffffffffff"
+                  ;"ffffffffffffffffffffffffff60010160005500"]
+     |>
+  else if a = n2w 0xa94f5374fce5edbc8e2a8697c15331677e6ebf0b then
+    <| nonce := 0x00
+     ; balance := 0x0ba1a9ce0ba1a9ce
+     ; storage := empty_storage
+     ; code := []
+     |>
+  else if a = n2w 0xcccccccccccccccccccccccccccccccccccccccc then
+    <| nonce := 0x00
+     ; balance := 0x0ba1a9ce0ba1a9ce
+     ; storage := empty_storage
+     ; code := hex_to_bytes "600060006000600060006004356110000162fffffff100"
+     |>
+  else empty_account_state
+End
+
+Definition add_d0g0v0_Shanghai_post_def:
+  add_d0g0v0_Shanghai_post a =
+  if a = n2w 0x0000000000000000000000000000000000001000 then
+    <| nonce := 0x00
+     ; balance := 0x0ba1a9ce0ba1a9ce
+     ; storage := (n2w 0x00 =+ n2w 0xfffffffffffffffffffffffffffffffffffffffffffffffffffffffffffffffe) empty_storage
+     ; code := hex_to_bytes $ CONCAT
+                 ["7ffffffffffffffffffffffffffffffffffffff"
+                 ;"fffffffffffffffffffffffffff7fffffffffff"
+                 ;"fffffffffffffffffffffffffffffffffffffff"
+                 ;"fffffffffffffff0160005500"]
+     |>
+  else if a = n2w 0x0000000000000000000000000000000000001001 then
+    <| nonce := 0x00
+     ; balance := 0x0ba1a9ce0ba1a9ce
+     ; storage := empty_storage
+     ; code := hex_to_bytes $ CONCAT
+                 ["60047fffffffffffffffffffffffffffffffffff"
+                 ;"ffffffffffffffffffffffffffffff0160005500"]
+     |>
+  else if a = n2w 0x0000000000000000000000000000000000001002 then
+    <| nonce := 0x00
+     ; balance := 0x0ba1a9ce0ba1a9ce
+     ; storage := empty_storage
+     ; code := hex_to_bytes $ CONCAT
+                 ["60017fffffffffffffffffffffffffffffffffff"
+                 ;"ffffffffffffffffffffffffffffff0160005500"]
+     |>
+  else if a = n2w 0x0000000000000000000000000000000000001003 then
+    <| nonce := 0x00
+     ; balance := 0x0ba1a9ce0ba1a9ce
+     ; storage := empty_storage
+     ; code := hex_to_bytes "600060000160005500"
+     |>
+  else if a = n2w 0x0000000000000000000000000000000000001004 then
+    <| nonce := 0x00
+     ; balance := 0x0ba1a9ce0ba1a9ce
+     ; storage := empty_storage
+     ; code := hex_to_bytes $ CONCAT
+                  ["7fffffffffffffffffffffffffffffffffffffff"
+                  ;"ffffffffffffffffffffffffff60010160005500"]
+     |>
+  else if a = n2w 0xa94f5374fce5edbc8e2a8697c15331677e6ebf0b then
+    <| nonce := 0x01
+     ; balance := 0x0ba1a9ce0b9aa781
+     ; storage := empty_storage
+     ; code := []
+     |>
+  else if a = n2w 0xcccccccccccccccccccccccccccccccccccccccc then
+    <| nonce := 0x00
+     ; balance := 0x0ba1a9ce0ba1a9cf
+     ; storage := empty_storage
+     ; code := hex_to_bytes "600060006000600060006004356110000162fffffff100"
+     |>
+  else empty_account_state
+End
+
+(*
 Definition CrashingTransaction_transaction_def:
   CrashingTransaction_transaction =
   <| from     := n2w 0xa94f5374fce5edbc8e2a8697c15331677e6ebf0b
@@ -29,5 +161,25 @@ Definition CrashingTransaction_transaction_def:
    ; accessList := []
    |>
 End
+secretKey = 0x45a915e4d060149eb4365960e6a7a45f334393093061116b197e3240065ff2d8
+
+Definition CrashingTransaction_pre_def:
+  CrashingTransaction_pre accounts ⇔
+  let account = accounts (n2w 0xa94f5374fce5edbc8e2a8697c15331677e6ebf0b) in
+    account.balance = 0x0de0b6b3a7640000 ∧
+    account.code = [] ∧
+    account.nonce = 0x0cc6 ∧
+    account.storage = K 0w
+End
+
+(*
+Definition CrashingTransaction_post_def:
+  CrashingTransaction_post r ⇔
+    state hash = n2w 0x7f2928f3c2a99e47eedce1880f49dbf3c44f9d304ec80bb7a14d755fae19a518
+    logs hash = n2w 0x1dcc4de8dec75d7aab85b567b6ccd41ad312451b948a7413f0a142fd40d49347
+
+                    "txbytes" : "0xf8c6820cc60b8347127a8001b87760606040525b5b61c3505a1115602c576040516034806039833901809050604051809103906000f0506006565b5b600a80606d6000396000f360606040525b3373ffffffffffffffffffffffffffffffffffffffff16ff5b600a80602a6000396000f360606040526008565b0060606040526008565b001ba0e3ff099a5b59f34c2e88fd6a42e44bf6ae186ebd06fa62aa18044da6a6d98df3a03efe897c69df0d45e18dd61580de2b700952cc9bc794fe05d0c6bf5e7f63d1d1"
+*)
+*)
 
 val _ = export_theory();
